Foundation/Modal/Kripke/Rooted.lean
@@ -1,0 +1,202 @@
+import Foundation.Modal.Kripke.Preservation
+
+namespace LO.Modal
+
+namespace Kripke
+
+open Formula.Kripke
+
+
+class Frame.Generated (F : Kripke.Frame) where
+  roots : Set F.World
+  roots_isRooted : ∀ w ∉ roots, ∃ r ∈ roots, r ≺^+ w
+
+class Frame.Rooted (F : Kripke.Frame) where
+  root : F.World
+  root_isPointRooted : ∀ w ≠ root, root ≺^+ w
+
+namespace PointRootedFrame
+
+
+variable {F : Frame}
+
+instance [rooted : F.Rooted] : F.Generated where
+  roots := {rooted.root}
+  roots_isRooted := by
+    rintro x hx;
+    use rooted.root;
+    constructor;
+    . tauto;
+    . exact rooted.root_isPointRooted x hx;
+
+end PointRootedFrame
+
+namespace Frame
+
+/-
+def setGenerate (F : Kripke.Frame) (R : Set F.World) (R_nonempty : R.Nonempty := by tauto_set) : Kripke.Frame where
+  World := { w // w ∈ R ∨ ∃ r ∈ R, r ≺^+ w }
+  Rel x y := x.1 ≺ y.1
+  world_nonempty := by
+    let ⟨r, hr⟩ := R_nonempty;
+    exact ⟨r, Or.inl hr⟩
+
+namespace setGenerate
+
+variable {F : Frame} {R : Set F.World} {R_nonempty : R.Nonempty}
+
+instance instGenerated : (F.setGenerate R R_nonempty).Generated where
+  roots := { r | r.1 ∈ R }
+  roots_isRooted := by
+    rintro ⟨x, (hr | ⟨r, hx₁, hx₂⟩)⟩ hw;
+    . simp at hw; contradiction;
+    . use ⟨r, by tauto⟩;
+      constructor;
+      . tauto;
+      . sorry;
+
+end setGenerate
+-/
+
+
+abbrev pointGenerate (F : Kripke.Frame) (r : F.World) : Kripke.Frame where
+  World := { w // w = r ∨ r ≺^+ w }
+  Rel x y := x.1 ≺ y.1
+  world_nonempty := ⟨r, by tauto⟩
+infix:100 "↾" => Frame.pointGenerate
+
+namespace pointGenerate
+
+open Relation
+
+variable {F : Frame} {r : F.World}
+
+lemma trans_rel_of_origin_trans_rel {hx : x = r ∨ r ≺^+ x} {hy : y = r ∨ r ≺^+ y} (Rxy : x ≺^+ y)
+  : (RelTransGen (F := F↾r) ⟨x, hx⟩ ⟨y, hy⟩) := by
+  induction Rxy using TransGen.head_induction_on with
+  | base h => exact Frame.RelTransGen.single h;
+  | @ih a c ha hb hc =>
+    let b : (F↾r).World := ⟨c, by
+      rcases hx with rfl | Rra <;>
+      rcases hy with rfl | Rrb;
+      . right; exact TransGen.single ha;
+      . right; exact TransGen.single ha;
+      . right; exact TransGen.tail Rra ha;
+      . right; exact TransGen.tail Rra ha;
+    ⟩;
+    apply Relation.TransGen.head (b := b);
+    . exact ha;
+    . apply hc;
+
+lemma origin_trans_rel_of_trans_rel {u v : (F↾r).World} (Ruv : u ≺^+ v) : u.1 ≺^+ v.1 := by
+  induction Ruv using TransGen.head_induction_on with
+  | base h => exact Frame.RelTransGen.single h;
+  | ih a b c => exact TransGen.head a c;
+
+-- set_option pp.proofs true in
+instance instPointRooted : (F↾r).Rooted where
+  root := ⟨r, by tauto⟩
+  root_isPointRooted := by
+    rintro ⟨w, (rfl | Rrw)⟩ hw;
+    . simp at hw;
+    . apply trans_rel_of_origin_trans_rel;
+      exact Rrw;
+
+instance [Finite F.World] : Finite (F↾r).World := Subtype.finite
+
+instance [DecidableEq F.World] : DecidableEq (F↾r).World := Subtype.instDecidableEq
+
+lemma rel_trans (F_trans : Transitive F) : Transitive (F↾r).Rel := by
+  rintro ⟨x, (rfl | hx)⟩ ⟨y, (rfl | hy)⟩ ⟨z, (rfl | hz)⟩ hxy hyz;
+  all_goals aesop;
+
+lemma rel_irrefl (F_irrefl : Irreflexive F) : Irreflexive (F↾r).Rel := by
+  rintro ⟨x, (rfl | hx)⟩ h;
+  all_goals aesop;
+
+/-
+lemma rel_universal_of_refl_eucl (F_refl : Reflexive F) (F_eucl : Euclidean F) : Universal (F↾r).Rel := by
+  have F_symm := symm_of_refl_eucl F_refl F_eucl;
+  rintro ⟨x, (rfl | hx)⟩ ⟨y, (rfl | hy)⟩;
+  . apply F_refl;
+  .
+    sorry;
+  . apply F_symm;
+    sorry;
+  . sorry;
+-/
+
+def generatedSub : F↾r ⥹ F where
+  toFun := λ ⟨x, _⟩ => x
+  forth := by
+    rintro ⟨x, (rfl | hx)⟩ ⟨y, (rfl | hy)⟩ hxy;
+    repeat exact hxy;
+  back := by
+    rintro ⟨x, (rfl | hx)⟩ y Rwv;
+    . simp at Rwv; use ⟨y, by tauto⟩
+    . use ⟨y, by right; exact Frame.RelTransGen.tail hx Rwv⟩;
+  monic := by simp;
+
+end pointGenerate
+
+end Frame
+
+
+class Model.Rooted (M : Kripke.Model) where
+  [frame_pointRooted : M.toFrame.Rooted]
+
+
+def Model.pointGenerate (M : Kripke.Model) (r : M.World) : Model where
+  toFrame := M.toFrame↾r
+  Val := λ w a => M.Val w.1 a
+infix:100 "↾" => Model.pointGenerate
+
+namespace Model.pointGenerate
+
+variable {M : Kripke.Model} {r : M.World}
+
+instance : (M↾r).Rooted where
+  frame_pointRooted := Frame.pointGenerate.instPointRooted
+
+instance : (M↾r) ⥹ M := by
+  letI g := Frame.pointGenerate.generatedSub (F := M.toFrame) (r := r);
+  exact {
+    toFun := g.toFun,
+    forth := g.forth,
+    back := g.back,
+    monic := g.monic
+    atomic := by
+      simp [Model.pointGenerate, Frame.pointGenerate, g];
+      rintro p x (rfl | Rrx) <;> tauto;
+  }
+
+def bisimulation_of_trans (r : M.World) : (M↾r) ⇄ M where
+  toRel x y := x.1 = y
+  atomic := by
+    rintro x y a rfl;
+    simp [Model.pointGenerate];
+  forth := by
+    rintro x₁ y₁ x₂ rfl Rx₂y₁;
+    use y₁.1;
+    constructor;
+    . simp;
+    . exact Rx₂y₁;
+  back := by
+    rintro ⟨x₁, (rfl | Rrx₁)⟩ x₂ y₂ rfl Rx₂y₂;
+    . use ⟨y₂, by right; exact Frame.RelTransGen.single Rx₂y₂⟩;
+      constructor;
+      . simp;
+      . exact Rx₂y₂;
+    . use ⟨y₂, (by right; exact Relation.TransGen.tail Rrx₁ Rx₂y₂;)⟩;
+      constructor;
+      . simp;
+      . exact Rx₂y₂;
+
+lemma modal_equivalent_at_root (r : M.World) : ModalEquivalent (M₁ := M↾r) (M₂ := M) ⟨r, by tauto⟩ r
+  := modal_equivalent_of_bisimilar (bisimulation_of_trans r) $ by simp [bisimulation_of_trans];
+
+end Model.pointGenerate
+
+end Kripke
+
+end LO.Modal
